some refinement.

Terms.v
@@ -13,6 +13,7 @@ Require Prerequistes.
 
 Module Make(Import M: Prerequistes.T).
 
+(** the core language of exceptions (L_exc) *)
  Inductive term: Type -> Type -> Type :=  
   | comp:   forall {X Y Z: Type}, term X Y -> term Y Z -> term X Z
   | copair: forall {X Y Z: Type}, term Z X -> term Z Y -> term Z (X+Y) 
@@ -24,11 +25,12 @@ Module Make(Import M: Prerequistes.T).
  Infix "o" := comp (at level 70).
 
  Definition id  {X: Type}       : term X X         := tpure id.
- Definition coproj1 {X Y}       : term (X+Y) X     := tpure inl.
- Definition coproj2 {X Y}       : term (X+Y) Y     := tpure inr.
- Definition emptyfun (X: Type) (e: Empty_set) : X := match e with end.
- Definition empty X: term X Empty_set := tpure (emptyfun X).
+ Definition in1 {X Y}       : term (X+Y) X         := tpure inl.
+ Definition in2 {X Y}       : term (X+Y) Y         := tpure inr.
+ Definition emptyfun (X: Type) (e: Empty_set) : X  := match e with end.
+ Definition empty X: (term X Empty_set)            := tpure (emptyfun X).
 
+(** programmer's language *)
  Inductive termpl: Type -> Type -> Type := 
   | pl_tpure: forall {X Y: Type}, (X -> Y) -> termpl Y X 
   | pl_comp: forall {X Y Z: Type}, termpl X Y -> termpl Y Z -> termpl X Z 
@@ -40,14 +42,14 @@ Module Make(Import M: Prerequistes.T).
  Definition pl_empty X: termpl X Empty_set := pl_tpure (emptyfun X).
  Definition pl_id {X: Type} : termpl X X := pl_tpure (Datatypes.id).
 
+(** translation from programmers' language into the core language *)
  Fixpoint translate X Y (t: termpl X Y): (term X Y) :=
   match t with
     | @pl_tpure X Y f      => tpure f
     | @pl_comp _ _ _ a b   => (translate _ _ a) o (translate _ _ b) 
     | @throw Y e           => (@empty Y) o (tag e)
-    | @try_catch X Y e a b => downcast(copair (@id Y) ((@translate _ _ b) o untag e) o coproj1 o (@translate _ _ a))
+    | @try_catch X Y e a b => downcast(copair (@id Y) ((@translate _ _ b) o untag e) o in1 o (@translate _ _ a))
   end.
-
 
 
 End Make.
