Derived_CoProjections.v
@@ -15,7 +15,7 @@ Set Implicit Arguments.
 Module Make(Import M: Prerequistes.T).
   Module Export Derived_CoProjectionsExp := Axioms.Make(M). 
 
- Definition permut {X Y} : term (X+Y) (Y+X) := copair coproj2 coproj1.
+ Definition permut {X Y} : term (X+Y) (Y+X) := copair in2 in1.
  Definition rcopair {X Y Z} (f: term X Y) (g: term X Z): term X (Y+Z) := copair g f o (@permut Z Y).
 
  Lemma is_permut X Y: EPURE (@permut X Y).
@@ -24,28 +24,28 @@ Module Make(Import M: Prerequistes.T).
 Lemma is_rcopair: forall k X Y Z (f1: term Z X) (f2: term Z Y), PPG f2 -> is k f1 -> is k f2 -> is k (rcopair f1 f2). (* FIXED *)
 Proof. intros k X Y Z f1 f2 H1 H2 H3. induction k; edecorate. Qed.
 
-Lemma s_rcopair_eq: forall X Z Y (f1: term X Y) (f2: term X Z), PPG f2 -> rcopair f1 f2 o coproj1 == f1.
+Lemma s_rcopair_eq: forall X Z Y (f1: term X Y) (f2: term X Z), PPG f2 -> rcopair f1 f2 o in1 == f1.
 Proof.
     intros X Y' Y f1 f2 H0. unfold rcopair, permut. rewrite <- assoc.
-    cut (copair coproj2 coproj1 o coproj1 == (@coproj2 Y' Y)).
+    cut (copair in2 in1 o in1 == (@in2 Y' Y)).
       intro H1. rewrite H1.
       apply s_lcopair_eq; exact H0.
       (*1st cut*)
       apply wtos; [edecorate| edecorate| ]. apply w_lcopair_eq; edecorate.
 Qed.
 
-Lemma w_rcopair_eq: forall X Z Y (f1: term X Y) (f2: term X Z), PPG f2 -> rcopair f1 f2 o coproj2 ~ f2.
+Lemma w_rcopair_eq: forall X Z Y (f1: term X Y) (f2: term X Z), PPG f2 -> rcopair f1 f2 o in2 ~ f2.
 Proof.
     intros X Y' Y f1 f2 H. unfold rcopair, permut. rewrite <- assoc.
     rewrite s_lcopair_eq;[| edecorate]. rewrite w_lcopair_eq;[reflexivity| edecorate].
 Qed.
 
 Lemma lcopair_u: forall X Y Y' (f1 f2: term X (Y' + Y)),
-  (f1 o coproj1 ~ f2 o coproj1) /\ (f1 o coproj2 == f2 o coproj2) -> f1 == f2.
+  (f1 o in1 ~ f2 o in1) /\ (f1 o in2 == f2 o in2) -> f1 == f2.
 Proof.
     intros X Y Y' f1 f2 (H0&H1). apply eeffect.
     (* f 1 ◦ [ ] ≡ f 2 ◦ [ ] *)
-    cut((@coproj2 Y' Y) o (@empty Y) == (@empty (Y' + Y))).
+    cut((@in2 Y' Y) o (@empty Y) == (@empty (Y' + Y))).
       intro H2. rewrite <- H2.
       setoid_rewrite assoc. rewrite H1. reflexivity. 
       (* 1st cut *)
@@ -55,11 +55,11 @@ Proof.
 Qed.
 
 Lemma rcopair_u: forall X Y Y' (f1 f2: term X (Y' + Y)),
-   (f1 o coproj1 == f2 o coproj1) /\ (f1 o coproj2 ~ f2 o coproj2) -> f1 == f2.
+   (f1 o in1 == f2 o in1) /\ (f1 o in2 ~ f2 o in2) -> f1 == f2.
 Proof.
      intros X Y Y' f1 f2 (H0&H1). apply eeffect.
      (* f 1 ◦ [ ] ≡ f 2 ◦ [ ] *)
-     cut((@coproj1 Y' Y) o (@empty Y') == (@empty (Y' + Y))).
+     cut((@in1 Y' Y) o (@empty Y') == (@empty (Y' + Y))).
        intro H2. rewrite <- H2.
        setoid_rewrite assoc. rewrite H0. reflexivity.
        (* 1st cut *)
