Proofs.v
@@ -4,7 +4,7 @@
 (*              (see file LICENSE for more details)                       *)
 (*                                                                        *)
 (*       Copyright 2015: Jean-Guillaume Dumas, Dominique Duval            *)
-(*			 Burak Ekici, Damien Pous.                        *)
+(*			 Burak Ekici, Damien Pous.                                        *)
 (**************************************************************************)
 
 Require Import Relations Morphisms.
@@ -17,7 +17,7 @@ Module Make(Import M: Prerequistes.T).
 
 
  (** Annihilation tag untag **)
- Lemma atu: forall e: EName, (tag e) o (untag e) == (@id Empty_set).
+ Lemma ATU: forall e: EName, (tag e) o (untag e) == (@id Empty_set).
  Proof.
     intro e.
     apply elocal_global.
@@ -33,14 +33,16 @@ Module Make(Import M: Prerequistes.T).
 Qed.
 
  (** Commutation untag untag **)
- Lemma cuu: forall (t s: EName) , s <> t -> 
-    (rcoprod (untag t) id) o coproj2 o (untag s) == (lcoprod id (untag s)) o coproj1 o (untag t).
+ Lemma CUUe: forall (t s: EName) , s <> t -> 
+    (rcoprod (untag t) id) o in2 o (untag s) ==
+    (lcoprod id (untag s)) o in1 o (untag t).
  Proof.
-    intros. apply elocal_global. intro r.  
+    intros. apply elocal_global. intro r.
     (* r = t /\ r <> s *)
-    destruct(Exc_dec r s). rewrite e. setoid_rewrite <- assoc at 4. rewrite (@eax2 s t); [| exact H].
+    destruct(Exc_dec r s). rewrite e. setoid_rewrite <- assoc at 4.
+      rewrite (@eax2 s t); [| exact H].
       setoid_rewrite <- assoc at 4. setoid_rewrite assoc at 2.
-      cut (coproj1 o (@empty (Val t)) == coproj2).
+      cut (in1 o (@empty (Val t)) == in2).
         intro H1. rewrite H1.
         rewrite assoc, s_lcoprod_eq; [| edecorate].
         setoid_rewrite <- assoc. rewrite eax1.
@@ -48,9 +50,10 @@ Qed.
         rewrite ids. reflexivity.
       (*1st cut*)
       setoid_rewrite s_empty; [reflexivity| edecorate| edecorate].
-     destruct(Exc_dec r t). rewrite e. setoid_rewrite <- assoc. rewrite (@eax2 t s); [| auto].
+    destruct(Exc_dec r t). rewrite e. setoid_rewrite <- assoc.
+       rewrite (@eax2 t s); [| auto].
        setoid_rewrite <- assoc. setoid_rewrite assoc at 2.
-        cut (coproj2 o (@empty (Val s)) == coproj1).
+        cut (in2 o (@empty (Val s)) == in1).
           intro H1. rewrite H1.
           rewrite assoc, s_rcoprod_eq; [| edecorate].
           setoid_rewrite <- assoc. rewrite eax1.
@@ -58,19 +61,21 @@ Qed.
           rewrite ids. reflexivity.
       (*2nd cut*)
       setoid_rewrite s_empty; [reflexivity| edecorate| edecorate].
-     setoid_rewrite <- assoc. rewrite (@eax2 r s); [| auto].
+    setoid_rewrite <- assoc. rewrite (@eax2 r s); [| auto].
        setoid_rewrite <- assoc. setoid_rewrite assoc at 2.
-        cut (coproj2 o (@empty (Val s)) == coproj1).
+        cut (in2 o (@empty (Val s)) == in1).
           intro H1. rewrite H1.
           rewrite assoc, s_rcoprod_eq; [| edecorate].
           setoid_rewrite <- assoc. 
           rewrite (@eax2 r t); [| auto].
           setoid_rewrite assoc at 3.
-          cut (coproj1 o (@empty (Val t)) == coproj2).
+          cut (in1 o (@empty (Val t)) == in2).
             intro H2. rewrite H2.
-            setoid_rewrite assoc at 2. rewrite s_lcoprod_eq; [| edecorate].
+            setoid_rewrite assoc at 2.
+            rewrite s_lcoprod_eq; [| edecorate].
             setoid_rewrite <- assoc. rewrite eax2; [| auto].
-            apply stow. setoid_rewrite assoc. apply replsubs; [| reflexivity].
+            apply stow. setoid_rewrite assoc.
+            apply replsubs; [| reflexivity].
             setoid_rewrite s_empty; [reflexivity| edecorate| edecorate].
           (*4th cut*)
           setoid_rewrite s_empty; [reflexivity| edecorate| edecorate]. 
@@ -78,21 +83,123 @@ Qed.
         setoid_rewrite s_empty; [reflexivity| edecorate| edecorate].
 Qed.
 
-(** PROVING AXIOMS OF PRGRAMMERS' LANGUAGE AFTER TRANSLATING THEM INTO THE CORE LANGUAGE **)
- Axiom mono: forall {X Y: Type} (f g: term Empty_set Y), PPG f /\ PPG g -> ((@empty X) o f == (@empty X) o g)-> f == g.
-
-
 (** propagate **)
-Lemma ppt: forall X Y (e: EName) (a: termpl Y X), PPG (translate _ _ a) ->
-                 (@translate _ _ (a O (@throw X e))) == (@translate _ _ (@throw Y e)). 
+ Lemma PPT: forall X Y (e: EName) (a: term Y X), PPG a ->
+            a o ((@empty X) o tag e) == (@empty Y) o tag e.
  Proof.
-    intros X Y e a H. simpl.
-    rewrite assoc. apply replsubs; [| reflexivity]. apply s_empty; edecorate.
+    intros X Y e a H.
+    rewrite assoc. apply replsubs; [| reflexivity].
+    apply s_empty; edecorate.
  Qed.
 
 
+(** PROVING AXIOMS OF PRGRAMMERS' 
+    LANGUAGE AFTER TRANSLATING THEM INTO THE CORE LANGUAGE **)
+ Axiom mono: forall {X Y: Type} (f g: term Empty_set Y), PPG f /\ PPG g -> 
+                                ((@empty X) o f == (@empty X) o g)-> f == g.
+
+(*recovery*)
+ Lemma RCV: forall X Y (e: EName) (u1 u2: term (Val e) Y), 
+            EPURE u1 -> EPURE u2 ->
+            ((@empty X) o tag e) o u1 == ((@empty X) o tag e) o u2 ->
+            u1 == u2.
+ Proof.
+    intros X Y e u1 u2 H0 H1 H2. setoid_rewrite <- assoc in H2.
+      apply mono in H2; [| split; apply is_comp; [edecorate| edecorate | edecorate | edecorate ]].
+      apply wtos; [edecorate| edecorate| ].
+        transitivity ((untag e o tag e) o u1).
+          + setoid_rewrite <- idt at 1.
+            apply pwsubs.
+            - symmetry. now rewrite eax1.
+            - unfold pure_id. split; easy.
+          + apply wsym. rewrite <- assoc, H2.
+            transitivity ((untag e o tag e) o u2).
+            - setoid_rewrite <- idt at 1.
+              apply pwsubs. now rewrite eax1.
+              unfold pure_id; split; easy.
+            - rewrite assoc. easy.
+ Qed.
+
+(** try **)
+ Lemma TRY: forall X Y (e: EName) (a1 a2: term Y X) (b: term Y (Val e)),  
+            PPG a1 -> PPG a2 ->  PPG b ->
+            a1 == a2 ->
+            downcast ((copair id (b o untag e) o in1) o a1) ==
+            downcast ((copair id (b o untag e) o in1) o a2).
+ Proof.
+    intros X Y e a1 a2 b H0 H1 H2 H3. simpl.
+      apply wtos; [edecorate| edecorate |].
+       setoid_rewrite <- w_downcast. rewrite H3.
+       reflexivity.
+ Qed.
+
+(*try0*)
+ Lemma TRY0: forall X Y (e: EName) (u: term Y X) (b: term Y (Val e)), EPURE u -> PPG b ->
+             downcast ((copair id (b o untag e) o in1) o u) == u.
+ Proof.
+    intros X Y e u b H0 H1.
+      apply wtos; [edecorate |edecorate| ].
+      rewrite <- w_downcast. 
+        transitivity(id o u).
+        apply pwsubs; [| split; [exact H0| reflexivity]].
+        apply w_lcopair_eq; edecorate.
+      rewrite idt. reflexivity.
+ Qed.
+
+(*try1*)
+ Lemma TRY1: forall X Y (e: EName) (u: term (Val e) X) (b: term Y (Val e)),
+             EPURE u -> PPG b ->
+             downcast ((copair id (b o untag e) o in1) o ((empty Y o tag e) o u)) == b o u.
+ Proof.
+    intros X Y e u b H0 H1.
+      apply wtos; [edecorate |edecorate| ].
+      rewrite <- w_downcast.
+      do 2 setoid_rewrite assoc.
+      setoid_rewrite <- assoc at 3.
+      cut (in2 == in1 o (@empty Y)).
+        intro H2. rewrite <- H2.
+        rewrite s_lcopair_eq; [| edecorate].
+        apply pwsubs; [| split; [exact H0| reflexivity]].
+        rewrite <- assoc. rewrite eax1, ids. reflexivity.
+      setoid_rewrite s_empty; [reflexivity| edecorate| edecorate].
+ Qed.
+
+ (** try2 **)
+Lemma TRY2: forall X Y e f (u: term (Val f) X) (b: term Y (Val e)),
+            e <> f -> EPURE u ->  PPG b ->
+            downcast ((copair id (b o untag e)) o in1 o (empty Y) o (tag f) o u) 
+            == (empty Y) o (tag f) o u.
+ Proof.
+    intros X Y e f u b H0 H1 H2. simpl.
+      apply wtos; [edecorate |edecorate| ].
+      rewrite <- w_downcast.
+      setoid_rewrite <- assoc at 3.
+      cut (in2 == in1 o (@empty Y)).
+        intro H3. rewrite <- H3.
+        rewrite s_lcopair_eq; [| edecorate].
+        apply pwsubs; [| split; [exact H1| reflexivity]].
+        rewrite <- assoc.
+        rewrite eax2; [| auto]. rewrite assoc.
+        cut((b o empty (Val e)) == empty Y).
+          intro H4. rewrite H4. reflexivity.
+        setoid_rewrite s_empty; [reflexivity| edecorate].
+      setoid_rewrite s_empty; [reflexivity| edecorate| edecorate].
+ Qed.
+
+
+(** the translation into the programmers' language *)
+
+(** propagate **)
+Lemma translated_ppt: forall X Y (e: EName) (a: termpl Y X), PPG (translate _ _ a) ->
+                      (@translate _ _ (a O (@throw X e))) == (@translate _ _ (@throw Y e)). 
+ Proof.
+    intros X Y e a H. simpl.
+    rewrite assoc. apply replsubs; [| reflexivity].
+    apply s_empty; edecorate.
+ Qed.
+
 (** recover **)
- Lemma rcv: forall X Y (e: EName) (u1 u2: termpl (Val e) Y), 
+ Lemma translated_rcv: forall X Y (e: EName) (u1 u2: termpl (Val e) Y), 
                EPURE (translate _ _ u1) -> EPURE (translate _ _ u2) ->
               (@translate _ _ ((@throw X e) O u1)) == (@translate _ _ ((@throw X e) O u2)) -> 
               (@translate _ _ u1) == (@translate _ _ u2).
@@ -112,7 +219,7 @@ Lemma ppt: forall X Y (e: EName) (a: termpl Y X), PPG (translate _ _ a) ->
  Qed.
 
 (** try **)
- Lemma try: forall X Y (e: EName) (a1 a2: termpl Y X) (b: termpl Y (Val e)),  
+ Lemma translated_try: forall X Y (e: EName) (a1 a2: termpl Y X) (b: termpl Y (Val e)),  
             PPG (translate _ _ a1) -> PPG (translate _ _ a2) ->  PPG (translate _ _ b) ->
             (translate _ _ a1) ==(translate _ _ a2) ->
             (@translate _ _ (try_catch e a1 b)) == (@translate _ _ (try_catch e a2 b)).
@@ -123,7 +230,7 @@ Lemma ppt: forall X Y (e: EName) (a: termpl Y X), PPG (translate _ _ a) ->
  Qed.
 
 (** try0 **)
- Lemma try0: forall X Y (e: EName) (u: termpl Y X) (b: termpl Y (Val e)),  
+ Lemma translated_try0: forall X Y (e: EName) (u: termpl Y X) (b: termpl Y (Val e)),  
              EPURE (translate _ _ u) -> PPG (translate _ _ b) ->
              (@translate _ _ (try_catch e u b)) == (@translate _ _ u).
  Proof.
@@ -136,7 +243,7 @@ Lemma ppt: forall X Y (e: EName) (a: termpl Y X), PPG (translate _ _ a) ->
  Qed.
 
 (** try1 **)
- Lemma try1: forall X Y (e: EName) (u: termpl (Val e) X) (b: termpl Y (Val e)),  
+ Lemma translated_try1: forall X Y (e: EName) (u: termpl (Val e) X) (b: termpl Y (Val e)),  
              EPURE (translate _ _ u) -> PPG (translate _ _ b) ->
              (@translate _ _ (try_catch e ((@throw Y e) O u) b)) == (@translate _ _ (b O u)).
  Proof.
@@ -144,7 +251,7 @@ Lemma ppt: forall X Y (e: EName) (a: termpl Y X), PPG (translate _ _ a) ->
       apply wtos; [edecorate |edecorate| ].
       rewrite <- w_downcast.
       do 2 setoid_rewrite assoc. setoid_rewrite <- assoc at 3.
-      cut (coproj2 == coproj1 o (@empty Y)).
+      cut (in2 == in1 o (@empty Y)).
         intro H2. rewrite <- H2.
         rewrite s_lcopair_eq; [| edecorate].
         apply pwsubs; [| split; [exact H0| reflexivity]].
@@ -153,7 +260,7 @@ Lemma ppt: forall X Y (e: EName) (a: termpl Y X), PPG (translate _ _ a) ->
  Qed.
 
  (** try2 **)
- Lemma try2: forall X Y e f (u: termpl (Val f) X) (b: termpl Y (Val e)),  e <> f -> 
+ Lemma translated_try2: forall X Y e f (u: termpl (Val f) X) (b: termpl Y (Val e)),  e <> f -> 
                 EPURE (translate _ _ u) ->  PPG (translate _ _ b) -> 
  		(@translate _ _ (try_catch e ((@throw Y f) O u) b))  == (@translate _ _ ((@throw Y f) O u)).
  Proof.
@@ -161,7 +268,7 @@ Lemma ppt: forall X Y (e: EName) (a: termpl Y X), PPG (translate _ _ a) ->
       apply wtos; [edecorate |edecorate| ].
       rewrite <- w_downcast.
       do 2 setoid_rewrite assoc. setoid_rewrite <- assoc at 3.
-      cut (coproj2 == coproj1 o (@empty Y)).
+      cut (in2 == in1 o (@empty Y)).
         intro H3. rewrite <- H3.
         rewrite s_lcopair_eq; [| edecorate].
         apply pwsubs; [| split; [exact H1| reflexivity]].
